aneris/examples/transactional_consistency/resource_algebras.v
@@ -49,6 +49,8 @@ Class IDBG Σ :=
     IDBG_Trace4 :> ghost_mapG Σ Key (option val);
     IDBG_Trace5 :> inG Σ (authR (gmapUR nat (agreeR (leibnizO transaction))));
     IDBG_Trace6 :> ghost_mapG Σ Key (list val);
+    IDBG_Trace7 :> ghost_mapG Σ socket_address (gname * gname * gname * val);
+    IDBG_Trace8 :> ghost_mapG Σ socket_address (option val);
   }.
 
 Notation KVSG Σ := (IDBG Σ).
@@ -75,6 +77,8 @@ Definition KVSΣ : gFunctors :=
      ghost_mapΣ Key (option val);
      GFunctor (authR (gmapUR nat (agreeR (leibnizO transaction))));
      ghost_mapΣ Key (list val);
+     ghost_mapΣ socket_address (gname * gname * gname * val);
+     ghost_mapΣ socket_address (option val);
      mono_natΣ;
      ras.SpecChanΣ;
      lockΣ].
